dimsum_examples/lam_examples.v
@@ -1,5 +1,5 @@
 From dimsum.core Require Export proof_techniques.
-From dimsum.core Require Import itree.
+From dimsum.core Require Import itree axioms.
 From dimsum.examples Require Import lam.
 
 Local Open Scope Z_scope.
@@ -11,6 +11,227 @@ Local Ltac go_s :=
 Local Ltac go_i :=
   tstep_i; go.
 
+Definition nb_itree: itree (moduleE lam_event unit) unit:= TNb.
+Lemma ub_itree_refines_everything s:
+  trefines (itree_mod nb_itree ()) s.
+Proof.
+  apply tsim_implies_trefines=>n. unfold nb_itree.
+  go_i. auto.
+Qed.
+
+(* ** Various Lam programs to test the TStepS and TStepI instances*)
+
+(* ** free variable*)
+Definition free_var_lam: fndef :={|
+fd_args := [];
+fd_body := Var "x";
+fd_static := I
+|}.
+Definition free_var_prog : gmap fid fndef :=
+  <[("free_var",None) := free_var_lam]> $ ∅.
+Definition free_var_mod := lam_mod free_var_prog.
+
+Definition free_var_itree : itree (moduleE lam_event unit) unit:=
+  h← TExist _;;;
+  TVis (Incoming, ELCall ("free_var",None) [] h);;;;
+  TUb.
+
+Lemma free_var_itree_refines_free_var_lam:
+  trefines (itree_mod free_var_itree ()) free_var_mod.
+Proof.
+  apply tsim_implies_trefines => n /=. unfold free_var_itree, free_var_prog. 
+  go_i. intros. go. go_i. go_s. left. eexists _,_,_. split!.
+  go_s. eexists _,_. split!. eauto. intros. auto.
+  unfold free_var_lam. simpl. go_s. auto. 
+Qed.
+
+
+(* ** Simple binary operation*)
+Definition add_lam: fndef :={|
+fd_args := ["x";"y"];
+fd_body := BinOp (Var "x") AddOp (Var "y");
+fd_static := I
+|}.
+Definition add_prog : gmap fid fndef :=
+  <[("add",None) := add_lam]> $ ∅.
+Definition add_mod := lam_mod add_prog.
+
+Definition add_itree : itree (moduleE lam_event unit) unit :=
+        '(f, vs, h) ← TReceive (λ '(f, vs, h), (Incoming, ELCall f vs h));;;
+        TAssume (f= ("add",None));;;;
+        x ← TAll _;;;
+        y ← TAll _;;; 
+        TAssume (vs = [ValNum x;ValNum y]);;;;
+        TVis (Outgoing, ELReturn (ValNum (x+y)) h);;;;
+        TUb.
+Lemma add_prog_refines_add_itree :
+  trefines add_mod (itree_mod add_itree ()).
+Proof.
+  apply tsim_implies_trefines => n. 
+  go_i. split!. intros. go_s. eexists (f, vs, h'). go.
+  go_s. split!. go. go_s. intros. go. go_s. intros. go.
+  go_s. intros. go. go_s. intros. go.
+  go_i. split!. unfold add_prog in *.  intros. 
+  rewrite lookup_insert_Some in H2.   destruct!. split!. go_i. go_i.
+  go_s. split!. go. go_s.  auto.
+  intros.
+  subst. rewrite lookup_insert_None in H2. destruct!.
+  intros. destruct!.
+Qed.
+
+Definition add_repeat_itree : itree (moduleE lam_event unit) unit :=
+        ITree.forever(
+          '(f, vs, h) ← TReceive (λ '(f, vs, h), (Incoming, ELCall f vs h));;;
+          TAssume (f= ("add",None));;;;
+          x ← TAll _;;;
+          y ← TAll _;;; 
+          TAssume (vs = [ValNum x;ValNum y]);;;;
+          TVis (Outgoing, ELReturn (ValNum (x+y)) h)
+        ) .
+Lemma add_prog_refines_add_repeat_itree :
+  trefines add_mod (itree_mod add_repeat_itree ()).
+Proof.
+  apply tsim_implies_trefines => n.
+  unshelve eapply tsim_remember.
+  { simpl. exact (λ _ σa '(t, _),
+  t ≈ add_repeat_itree ∧
+  ∃h, σa= Lam Waiting [] h add_prog). } 
+  {simpl. naive_solver. }
+  { simpl. eauto. }
+  { simpl. intros ???[????][??][??]. destruct!. 
+  go_i. split!. intros. go_s. go_s. rewrite -/add_repeat_itree. eexists (f, vs, h'). go.
+  go_s. intros. split. naive_solver. go. go_s. intros. go. go_s. intros.
+  go. go_s. intros. go. go_s. intros. go. go_i. split.
+  intros. unfold add_prog. rewrite lookup_insert_Some in H5. destruct!/=; subst.
+  split!. go_i. go_i. go_s. split!. go. 
+  eapply H0; auto. split!. naive_solver.
+  intros. destruct!. }
+Qed. 
+
+Definition add_wrong_lam: fndef :={|
+fd_args := [];
+fd_body := BinOp (Val (ValNum 0)) AddOp (Val (ValBool true));
+fd_static := I
+|}.
+Definition add_wrong_prog : gmap fid fndef :=
+  <[("add_wrong",None) := add_wrong_lam]> $ ∅.
+Definition add_wrong_mod := lam_mod add_wrong_prog.
+Definition add_wrong_itree : itree (moduleE lam_event unit) unit:=
+  h← TExist _;;;
+  TVis (Incoming, ELCall ("add_wrong",None) [] h);;;;
+  TUb.
+
+Lemma add_wrong_itree_refines_add_wrong_lam:
+  trefines (itree_mod  add_wrong_itree ()) add_wrong_mod.
+Proof.
+  apply tsim_implies_trefines => n.
+  go_i. intros. go. go_i. 
+  go_s. left.
+  eexists ("add_wrong", None),[],x.
+  split!. 
+  go_s. eexists _,_. split!. rewrite lookup_insert_Some. left. auto. intros.
+  auto. go_s. intros. inversion H1.
+Qed.  
+
+(* ** newrefs *)
+Definition newref_lam: fndef :={|
+fd_args := ["x";"y"];
+fd_body := NewRef (Var "x") (Var "y");
+fd_static := I
+|}.
+Definition newref_prog : gmap fid fndef :=
+  <[("newref",None) := newref_lam]> $ ∅.
+Definition newref_mod := lam_mod newref_prog.
+
+Definition newref_itree : itree (moduleE lam_event unit) unit :=
+    ITree.forever(
+      '(f, vs, h) ← TReceive (λ '(f, vs, h), (Incoming, ELCall f vs h));;;
+      TAssume (f= ("newref",None));;;;
+      x ← TAll _;;;
+      y ← TAll _;;; 
+      TAssume (vs = [ValNum x;ValNum y]);;;;
+      TAssume (y>0);;;;
+      l ← TExist _;;;
+      h' ← TExist _;;;
+      TVis (Outgoing, ELReturn (ValLoc l) h');;;;
+      (* ** add assertions*)
+      TAssert( h'.(h_heap)!!l = Some (ValNum x))
+    ) .
+Lemma newref_prog_refines_newref_itree :
+  trefines newref_mod (itree_mod newref_itree ()).
+Proof.
+  apply tsim_implies_trefines => n.
+  unshelve eapply tsim_remember.
+  { simpl. exact (λ _ σa '(t, _),
+  t ≈ newref_itree ∧
+  ∃h, σa= Lam Waiting [] h newref_prog). }
+  {naive_solver. }
+  {naive_solver. }
+  intros ???[????][??][?[??]]. inversion H2; subst.
+  go_i. split!.
+  - intros. go_s. go_s. exists (f, vs, h'). go. go_s. split!. go.
+  go_s. intros. go. go_s. intros. go. go_s. intros. go. go_s. intros. destruct!. go. go_s. intros. go.
+  go_i. split!. intros. rewrite lookup_insert_Some in H4. destruct!. split!. 
+  (* ** newref part *)
+  go_i. intros. split!.
+  go_s. exists l. go. go_s. exists h'0. go. go_i. go_s. split!.
+  go. go_s.
+  split!. unfold heap_alloc_prop in H4. destruct!. inversion H2. apply heap_alloc_h_lookup. lia. lia.
+  rewrite -/newref_itree. go. apply H0. auto. split!. 
+  - intros. destruct!.
+Qed.
+   
+Definition newref_nonnum_lam: fndef :={|
+fd_args := [];
+fd_body := NewRef (Val (ValNum 0)) (Val(ValBool true));
+fd_static := I
+|}.
+Definition newref_nonnum_prog : gmap fid fndef :=
+  <[("newref_nonnum",None) := newref_nonnum_lam]> $ ∅.
+Definition newref_nonnum_mod := lam_mod newref_nonnum_prog.
+
+Definition newref_nonnum_itree : itree (moduleE lam_event unit) unit :=
+  h← TExist _;;;
+  TVis (Incoming, ELCall ("newref_nonnum",None) [] h);;;;
+  TUb.
+Lemma newref_nonnum_itree_refines_newref_nonnum_lam:
+  trefines (itree_mod newref_nonnum_itree ()) newref_nonnum_mod.
+Proof.
+  apply tsim_implies_trefines => n.
+  go_i. intros. go. go_i. 
+  go_s. left.
+  eexists ("newref_nonnum", None),[],x.
+  split!. 
+  go_s. eexists _,_. split!. rewrite lookup_insert_Some. left. auto. intros.
+  auto. go_s. exists (0,0). exists ∅.  
+  split!. 
+Qed.
+
+Definition newref_zero_lam: fndef :={|
+fd_args := [];
+fd_body := NewRef (Val (ValNum 0)) (Val (ValNum 0));
+fd_static := I
+|}.
+Definition newref_zero_prog : gmap fid fndef :=
+  <[("newref_zero",None) := newref_zero_lam]> $ ∅.
+Definition newref_zero_mod := lam_mod newref_zero_prog.
+
+Definition newref_zero_itree : itree (moduleE lam_event unit) unit :=
+  h← TExist _;;;
+  TVis (Incoming, ELCall ("newref_zero",None) [] h);;;;
+  TUb.
+Lemma newref_zero_itree_refines_newref_zero_lam:
+  trefines (itree_mod newref_zero_itree ()) newref_zero_mod.
+Proof.
+  apply tsim_implies_trefines => n.
+  go_i. intros. go. go_i. go_s. left.
+  eexists ("newref_zero", None),[],x.
+  split!. 
+  go_s. split!. rewrite lookup_insert_Some. left. auto. 
+  auto. intros. go_s.
+  eexists (0,0),∅. intros. destruct!.  split!. left. reflexivity.
+Qed. 
+
 
 (* ** identity function*)
 Definition id_lam: fndef := {|
@@ -20,43 +241,415 @@ Definition id_lam: fndef := {|
 |}.
 Definition id_prog : gmap fid fndef :=
   <[("id",None) := id_lam]> $ ∅.
-
 Definition id_mod := lam_mod id_prog.
 
 (* ** identity specification*)
-Definition id_itree : itree (moduleE lam_event (list fid)) unit :=
-    ITree.forever (
+Definition id_simple_itree : itree (moduleE lam_event (list fid)) unit :=
         '(f, vs, h) ← TReceive (λ '(f, vs, h), (Incoming, ELCall f vs h));;;
         fid_list ← TGet ;;;
-        if bool_decide (f = ("id",None)) then
-          newfid ← TExist fid;;;
-          TPut (newfid::fid_list);;;;
-          TVis (Outgoing, ELReturn (ValFid newfid) h)
-        else if bool_decide (f ∈ fid_list) then
-          z ← TAll Z;;;
-          TAssume (vs = [ValNum z]);;;;
-          TVis (Outgoing, ELReturn (ValNum z) h)
-        else
-          TNb).
+        TAssume (f = ("id",None));;;;
+        TAssume (vs = []);;;;
+        newfid ← TExist fid;;;
+        TPut (newfid::fid_list);;;;
+        TVis (Outgoing, ELReturn (ValFid newfid) h);;;;
+        '(f, vs, h) ← TReceive (λ '(f, vs, h), (Incoming, ELCall f vs h));;;
+        fid_list ← TGet ;;;
+        TAssume (f ∈ fid_list);;;;
+        z ← TAll Z;;;
+        TAssume (vs = [ValNum z]);;;;
+        TVis (Outgoing, ELReturn (ValNum z) h);;;;
+        TUb.
 
-Lemma id_prog_refines_id_itree :
-  trefines id_mod (itree_mod id_itree []).
+Lemma id_prog_refines_id_simple_itree :
+  trefines id_mod (itree_mod id_simple_itree []).
 Proof.
     apply tsim_implies_trefines => n0 /=. unfold id_prog.
     tstep_i;  split; intros.
-    - admit. 
-    - admit.
+    - go_s. exists (f,vs,h'). go. go_s. split!. go. go_s. go_s. intros. go.
+    go_s. intros. go. go_i. split!.
+      { intros. split!. subst. rewrite lookup_insert_Some in H2. destruct!. reflexivity.
+      rewrite lookup_insert_Some in H2. destruct!. go_i. intros. split!.
+      go_s. exists ("id", Some n). go. go_s. go_i. go_s. split!.
+      go. go_i. split;intros. 
+        - go_s. exists (f, vs, h'0). go. go_s. split!. go. go_s.
+        go_s. intros. go. go_s. intros. go. go_s. intros. go.
+        go_i. split.
+        *  intros. rewrite elem_of_cons in H2. destruct!. rewrite lookup_insert_Some in H4. destruct!.
+        split!. go_i. go_s. split!. go. go_s. auto. apply elem_of_nil in H2. inversion H2. 
+        * intros. rewrite lookup_insert_None in H4. destruct!. rewrite elem_of_cons in H2. destruct!.
+        apply elem_of_nil in H2. inversion H2. 
+        - destruct!.  
+      }
+      {intros.  rewrite lookup_insert_None in H2. destruct!. } 
+    - destruct!. 
+    Unshelve. auto.
+Qed.
 
+Definition id_loop_itree : itree (moduleE lam_event (list fid)) unit :=
+  ITree.forever(
+        '(f, vs, h) ← TReceive (λ '(f, vs, h), (Incoming, ELCall f vs h));;;
+        fid_list ← TGet ;;;
+        if (bool_decide(f = ("id",None)))
+          then 
+          TAssume (vs = []);;;;
+          newfid ← TExist fid;;;
+          TPut (newfid::fid_list);;;;
+          TVis (Outgoing, ELReturn (ValFid newfid) h)
+        else if (bool_decide(f∈fid_list))
+          then 
+          z ← TAll Z;;;
+          TAssume (vs = [ValNum z]);;;;
+          TVis (Outgoing, ELReturn (ValNum z) h)
+        else TUb
+  ).
+
+Fixpoint fns_add_list fns l entry:=
+  match l with 
+    | [] => fns 
+    | hd::tl => fns_add (fns_add_list fns tl entry) hd entry
+    end.  
+
+Lemma lookup_add_list_None m l entry f: fns_add_list m l entry !! f= None → m !! f = None.
+Proof.
+  induction l.
+  auto.
+  simpl. intros. rewrite lookup_insert_None in H. destruct!. auto.
+Qed.
+
+Lemma lookup_add_list_in m l entry f: f∈l→fns_add_list m l entry !! f= Some entry .
+Proof.
+  induction l.
+  auto.
+  simpl. intros. apply elem_of_nil in H. inversion H. 
+  intros. apply elem_of_cons in H. destruct!. simpl.
+  rewrite lookup_insert_Some . split!. simpl.
+  rewrite lookup_insert_Some. destruct (bool_decide(a=f)) eqn:K.
+  case_bool_decide. left. auto. inversion K. case_bool_decide. inversion K.
+  right. naive_solver. 
+Qed.
+
+Lemma lookup_add_list_not_in m l entry f: f∉l→fns_add_list m l entry !! f= m !! f .
+Proof.
+  induction l.
+  auto.
+  simpl. intros. rewrite not_elem_of_cons in H. destruct!.
+  apply IHl in H1. rewrite -H1. rewrite lookup_insert_ne. reflexivity. intro. subst. contradiction. 
+Qed.
+
+Lemma id_prog_refines_id_loop_itree :
+  trefines id_mod (itree_mod id_loop_itree []).
+Proof.
+  apply tsim_implies_trefines => n0 /=.
+  unshelve eapply tsim_remember.
+  {simpl. exact (λ _ σa '(t, l),
+  t ≈ id_loop_itree ∧
+  ∃h id_prog', σa= Lam Waiting [] h id_prog'/\ 
+  id_prog' = fns_add_list id_prog l (Build_fndef ["x"] (Var "x") I) /\ 
+  ("id",None)∉l). }
+  {simpl. split!. reflexivity. intro. apply elem_of_nil in H. auto. }
+  {simpl. intros. destruct!. split!. }
+  {simpl. intros. destruct!.
+
+  go_i. split!;[|intros;destruct!]. intros. go_s. go_s. exists (f,vs,h'). go.
+  go_s. split!. go. go_s. case_bool_decide. 
+  - (* f = ("id", None)*)
+   go_s. intros. go. 
+   go_i. split!.
+   * intros. 
+   rewrite lookup_add_list_not_in in H6; [|naive_solver]. rewrite lookup_insert_Some in H6.
+   destruct!. split!.
+   go_i. intros. exists I. go_i. go_s. exists ("id", Some n). go.
+   go_s. go_s. split!.  rewrite -/id_loop_itree. go. apply H0. auto. split!.
+   rewrite not_elem_of_cons. split!.
+   * intros.  apply lookup_add_list_None in H6. rewrite lookup_insert_None in H6. destruct!.
+  - case_bool_decide.
+   * (* f = ("id", Some n)*)
+    go_s. intros. go. go_s. intros. go.  go_i. split!.
+    + intros. rewrite lookup_add_list_in in H7; auto. inversion H7. split!. naive_solver. subst.
+    go_i. go_s. rewrite -/id_loop_itree. split!. go. apply H0. auto.
+    split!. 
+    + intros. apply (lookup_add_list_in id_prog l (Build_fndef ["x"] (Var "x") I)) in H4.
+    rewrite H4 in H7. inversion H7. 
+   * go_s. auto.  
+  }
+  Qed. 
+
+(* ** recursive identity function*)
+Definition rec_id_lam: fndef := {|
+  fd_args := [];
+  fd_body := FixE "f" ["x"] (
+    If (BinOp (Var "x") EqOp (Val 0)) 
+    (Val 0)
+    (BinOp (Val 1) AddOp (App (Var "f") ([BinOp (Var "x") AddOp (Val (-1))])))
+  );
+  fd_static := I
+|}.
+Definition rec_id_prog : gmap fid fndef :=
+  <[("rec_id",None) := rec_id_lam]> $ ∅.
+Definition rec_id_mod := lam_mod rec_id_prog.
+
+Definition rec_id_loop_itree : itree (moduleE lam_event (gmap fid unit)) unit :=
+  ITree.forever(
+        '(f, vs, h) ← TReceive (λ '(f, vs, h), (Incoming, ELCall f vs h));;;
+        fid_map ← TGet ;;;
+        if (bool_decide(f = ("rec_id",None)))
+          then 
+          TAssume (vs = []);;;;
+          newfid ← TExist fid;;;
+          TPut (insert newfid () fid_map);;;;
+          TVis (Outgoing, ELReturn (ValFid newfid) h)
+        else if (bool_decide(f∈dom fid_map))
+          then 
+          z ← TAll Z;;;
+          TAssume (vs = [ValNum z]);;;;
+          TAssume (z>=0);;;;
+          TVis (Outgoing, ELReturn (ValNum z) h)
+        else TUb
+  ).
+
+Program Definition rec_id_prop elem key := 
+  match elem with 
+  | Some e => 
+    e = Build_fndef ["x"] 
+    (If (BinOp (Var "x") EqOp (Val 0)) 
+    (Val 0)
+    (BinOp (Val 1) AddOp (App (Val (ValFid key)) ([BinOp (Var "x") AddOp (Val (-1))])))) 
+    _
+  | _ => False
+  end
+.
+Next Obligation. intros. simpl. destruct key. destruct o; auto.
+Qed.
+
+
+Lemma rec_id_map_forall_neq k (m:gmap _ unit) entry p: k ∉dom m → map_Forall
+(λ (key : fid) (_ : ()), rec_id_prop (p !! key) key) m →
+map_Forall (λ (key : fid) (_ : ()), rec_id_prop 
+(fns_add p k entry !! key) key) m.
+Proof.
+  intros.
+  assert (map_Forall (λ (key : fid) (_ : ()), k≠key/\rec_id_prop (p !! key) key) m).
+  apply map_Forall_lookup_2.
+  intros.
+  split!.
+  intro; subst. rewrite not_elem_of_dom in H. rewrite H1 in H. inversion H.
+  rewrite  map_Forall_lookup in H0.
+  eapply H0. exact H1.
+  eapply map_Forall_impl.
+  exact H1.
+  simpl.
+  intros.
+  rewrite lookup_insert_ne; by destruct!.
+Qed.
+  
+Lemma rec_id_fundamental_lemma x prog f n' Ks h': 
+  0<=x→
+  prog !! f =
+  Some
+    (Build_fndef ["x"]
+       (If (BinOp (Var "x") EqOp (Val 0)) (Val 0)
+          (BinOp (Val 1) AddOp
+             (App (Val (ValFid f)) [BinOp (Var "x") AddOp (Val (-1))])))
+       (rec_id_prop_obligation_1 f))→
+  Lam
+  (expr_fill Ks
+     (If (BinOp (Val x) EqOp (Val 0)) (Val 0)
+        (BinOp (Val 1) AddOp
+           (App (Val (ValFid f)) [BinOp (Val x) AddOp (Val (-1))])))) [f.1]
+  h' prog ⪯{lam_trans, lam_trans, n', true} 
+  Lam
+  (expr_fill Ks  (Val x)) [f.1]
+  h' prog 
+.
+Proof.
+  intros.
+  generalize dependent Ks.
+  remember (λ x,∀ Ks,
+  Lam(expr_fill Ks
+     (If (BinOp (Val x) EqOp (Val 0)) (Val 0)
+        (BinOp (Val 1) AddOp
+           (App (Val (ValFid f)) [BinOp (Val x) AddOp (Val (-1))])))) [f.1]
+  h' prog ⪯{lam_trans, lam_trans, n', true} 
+  Lam (expr_fill Ks  (Val x)) [f.1] h' prog ).
+  remember (natlike_rec P).
+  clear Heqp. subst.
+  apply p; auto.
+  - intros. go_i. split!. go_i. apply trefines_implies_tsim. reflexivity. (* reflexive*)
+  - intros. go_i. split!. go_i. case_bool_decide. assert (~0 ≤ x0) by lia. contradiction.
+    go_i. 
+    assert (Z.succ x0 + -1 = x0) by lia.
+    rewrite H4.
+    go_i.
+    split!.
+    intros. rewrite H0 in H5. inversion H5. split!.
+    assert (∀e, expr_fill Ks (BinOp (Val 1) AddOp e) = expr_fill ((BinOpRCtx 1 AddOp)::Ks) e) by auto.
+    rewrite H6.
+    apply trefines_implies_tsim.
+    admit. (*transitive*)
+  intros.
+  rewrite H5 in H0.
+  inversion H0.
 Admitted.
 
 
+Lemma rec_id_prog_refines_rec_id_loop_itree :
+  trefines rec_id_mod (itree_mod rec_id_loop_itree ∅).
+Proof.
+  apply tsim_implies_trefines => n0 /=.
+  unshelve eapply tsim_remember.
+  {simpl. 
+  exact (λ _ σa '(t, m),
+  t ≈ rec_id_loop_itree ∧
+  ∃h rec_id_prog', σa= Lam Waiting [] h rec_id_prog'/\ 
+  map_Forall (λ key _, rec_id_prop (rec_id_prog' !! key ) key)  m/\ 
+  ("rec_id",None)∉ dom m/\ 
+  rec_id_prog!!("rec_id",None)=rec_id_prog'!!("rec_id",None)). }
+  {simpl. split!. reflexivity.  intro. intros. rewrite lookup_empty in H. inversion H. auto.  }
+  {simpl. intros. destruct!. split!. }
+  {simpl. intros. destruct!.
 
+  go_i. split!;[|intros;destruct!]. intros. go_s. go_s. exists (f,vs,h'). go.
+  go_s. split!. go. go_s. case_bool_decide.
+  - (* f = ("rec_id", None)*)
+   go_s. intros. go. 
+   go_i. split!.
+   * intros.  subst. rewrite -H6 in H8. rewrite lookup_insert_Some in H8. destruct!.
+   split!. go_i. intros. exists I. go_i. go_s. rewrite -/rec_id_loop_itree. exists ("rec_id", Some n).
+   go. go_s. go_s. split!. go. apply H0; auto. split!.  apply map_Forall_insert_2.
+    + (*prove rec_id_prop*) rewrite lookup_insert. split!. f_equal. apply AxProofIrrelevance . 
+    + apply rec_id_map_forall_neq; auto. 
+    intro. rewrite map_Forall_lookup in H3. rewrite elem_of_dom in H7. unfold is_Some in H7. destruct!.
+    apply H3 in H7. unfold rec_id_prop in H7. rewrite H5 in H7. auto.
+    + rewrite not_elem_of_dom. rewrite lookup_insert_None; split!. by rewrite - not_elem_of_dom.
+    +  rewrite (lookup_insert_ne _ ("rec_id", Some n)). auto. auto. 
+   * intros. subst. rewrite -H6 in H8.   rewrite lookup_insert_None in H8. destruct!.
+  - case_bool_decide.
+   * (* f = ("rec_id", Some n)*)
+    go_s. intros. go. go_s. intros. go.  go_i. split!.
+    + intros. rewrite elem_of_dom in H7. destruct H7. rewrite map_Forall_lookup in H3.
+    apply H3 in H7. rewrite H9 in H7. unfold rec_id_prop in H7. subst. split!. 
+    go_s. intros. rewrite -/rec_id_loop_itree. go.
 
-    unshelve eapply tsim_remember. 
-    { simpl. exact (λ _ σa '(t, _),
-    t ≈ id_itree ∧
-    σa.(asm_cur_instr) = AWaiting ∧
-    σa.(asm_instrs) = print_asm).  }
+    (* ** main theorem!!*)
+    assert (∀e, ReturnExt e = expr_fill [ReturnExtCtx] e).
+    auto.
+    rewrite H8.
+    
+    admit.
+    + intros. rewrite elem_of_dom in H1. destruct H1. rewrite H9 in H1. inversion H1. 
+   * go_s. auto.  
+  }
+  Admitted.
+  
+
+(* ** closure add*)
+Definition clos_add_lam: fndef :={|
+fd_args := [];
+fd_body := 
+  FixE "" ["x"] (
+    FixE "" ["y"] (
+      BinOp (Var "x") AddOp (Var "y")
+    )
+);
+fd_static := I
+|}.
+Definition clos_add_prog : gmap fid fndef :=
+  <[("clos_add",None) := clos_add_lam]> $ ∅.
+Definition clos_add_mod := lam_mod clos_add_prog.
+
+Inductive clos_add_ctype:=
+  | Main
+  | Initial 
+  | Final (z:Z).
+
+Definition clos_add_loop_itree : itree (moduleE lam_event (gmap fid clos_add_ctype)) unit :=
+  ITree.forever(
+        '(f, vs, h) ← TReceive (λ '(f, vs, h), (Incoming, ELCall f vs h));;;
+        fid_map ← TGet ;;;
+        match fid_map !! f with 
+          | Some Main => 
+            TAssume (vs = []);;;;
+            newfid ← TExist fid;;;
+            TPut (insert newfid Initial fid_map);;;;
+            TVis (Outgoing, ELReturn (ValFid newfid) h)
+          | Some Initial => 
+            x ← TAll _;;;
+            TAssume (vs = [ValNum x]);;;;
+            newfid ← TExist fid;;;
+            TPut (insert newfid (Final x) fid_map);;;;
+            TVis (Outgoing, ELReturn (ValFid newfid) h)
+          | Some (Final x) =>  
+            y ← TAll _;;;
+            TAssume (vs = [ValNum y]);;;;
+            TVis (Outgoing, ELReturn (ValNum (x+y)) h)
+          | None => TUb 
+        end
+  ).
+
+Definition clos_add_fns_m_prop (fns:gmap fid fndef) (m:gmap fid clos_add_ctype):Prop:= 
+  ∀ f:fid, 
+  (fns!!f = Some clos_add_lam ↔ m!!f = Some Main)/\ 
+  (fns!!f = Some {|
+    fd_args := ["x"];
+    fd_body := 
+      FixE "" ["y"] (
+        BinOp (Var "x") AddOp (Var "y")
+      )
+    ;
+    fd_static := I
+    |} ↔ m!!f = Some Initial)/\ 
+    (∀n, fns!!f = Some {|
+    fd_args := ["y"];
+    fd_body := 
+      BinOp (Val (ValNum n)) AddOp (Var "y")
+    ;
+    fd_static := I
+    |} ↔ m!!f = Some (Final n))
+  .
+
+Lemma clos_add_prog_refines_clos_add_loop_itree :
+  trefines clos_add_mod (itree_mod clos_add_loop_itree (insert ("clos_add",None) Main ∅)).
+Proof.
+  apply tsim_implies_trefines. intros.
+  unshelve eapply tsim_remember.
+  {simpl. exact (λ n s '(t,m),
+    t ≈ clos_add_loop_itree ∧
+    ∃h fns, s= Lam Waiting [] h fns ∧
+    clos_add_fns_m_prop fns m
+    ). }
+  {simpl. split!. reflexivity. unfold clos_add_fns_m_prop. intros. split!; split; intros;
+   rewrite lookup_insert_Some in H;rewrite lookup_insert_Some;naive_solver. }
+  {simpl. intros. auto. }
+  {simpl. intros. destruct!. go_i. split!.
+   {intros. go_s. go_s. rewrite -/clos_add_loop_itree. exists (f, vs, h'). go. go_s. split!. go. go_s.
+    destruct (m!!f) eqn:V.  unfold clos_add_fns_m_prop in H4. remember (H4 f). destruct!. clear Heqa.
+    - destruct c eqn:V'.
+      + (* main case*) go_s. intros. go. go_i. split!; intros. 
+        * rewrite- H3 in V. rewrite H8 in V. inversion V. subst. split!.
+          go_i. intros. exists I. go_i. go_s. exists (f.1, Some n0). go. go_s. go_s. split!. go.
+          apply H0. auto. split!.  
+          unfold clos_add_fns_m_prop. 
+          intros;split!; split;intros; 
+          rewrite lookup_insert_Some in H9; rewrite lookup_insert_Some; naive_solver.
+        * rewrite -H3 in V. rewrite H8 in V. inversion V.   
+      + (* Initial case*)  go_s. intros. go. go_s. intros. go. go_i. split!; intros. 
+        * rewrite -H6 in V. rewrite H8 in V. inversion V. subst. split!. 
+        go_i. intros. exists I. go_i. go_s. exists (f.1, Some n0). go. go_s. go_s. split!. go. apply H0.
+        auto. split!.
+        unfold clos_add_fns_m_prop. 
+        intros;split!; split;intros; 
+        rewrite lookup_insert_Some in H9; rewrite lookup_insert_Some; naive_solver.
+        * rewrite -H6 in V. rewrite H8 in V. inversion V.  
+      + (* Final case*) go_s. intros. go. go_s. intros. go. go_i. split!; intros. 
+        * rewrite -H7 in V. rewrite H8 in V. inversion V. subst. split!.
+          go_i. go_i. go_s. split!. go. apply H0. auto. split!. 
+        * rewrite -H7 in V. rewrite H8 in V. inversion V.  
+    - go_s. auto. 
+   } 
+   {intros. destruct!. }
+  }
+Qed.
+
 
 Definition main_lam: fndef := {|
   fd_args := ["input"];
